Run a test case for ArrayTest, debugging byte operations of AMD64_gas in the process

platform/tests/ArrayTest.v
@@ -1,4 +1,4 @@
-Require Import Arith AutoSep.
+Require Import Arith AutoSep Malloc.
 
 
 Definition readS := SPEC("arr", "pos") reserving 0
@@ -26,7 +26,20 @@ Definition sumS := SPEC("arr", "len") reserving 3
   PRE[V] array8 arr (V "arr") * [| V "len" = length arr |] * [| goodSize (length arr) |]
   POST[R] array8 arr (V "arr") * [| R = sum arr |].
 
-Definition m := bmodule "array" {{
+Definition testS := SPEC reserving 9
+  PREonly[_] mallocHeap 0.
+
+Inductive please_materialize (sz : nat) : Prop := PleaseMaterialize.
+Hint Constructors please_materialize.
+
+Definition array8_decomission (sz : nat) := array8.
+
+Definition decomission_ok (sz : nat) (bs : list B) :=
+  length bs = sz * 4.
+
+Definition m := bimport [[ "malloc"!"malloc" @ [mallocS], "malloc"!"free" @ [freeS],
+                           "sys"!"abort" @ [abortS], "sys"!"printInt" @ [printIntS] ]]
+  bmodule "array" {{
   bfunction "read"("arr", "pos") [readS]
     "arr" <-*8 "arr" + "pos";;
     Return "arr"
@@ -65,6 +78,52 @@ Definition m := bmodule "array" {{
     };;
 
     Return "acc"
+  end with bfunctionNoRet "test"("arr", "tmp") [testS]
+    "arr" <-- Call "malloc"!"malloc"(0, 2)
+    [PREonly[_, R] mallocHeap 0 * R =?> 2 * [| R <> 0 |] * [| freeable R 2 |] ];;
+
+    Note [please_materialize 2];;
+
+    Assert [Al arr,
+      PREonly[V] mallocHeap 0 * [| V "arr" <> 0 |] * [| freeable (V "arr") 2 |]
+        * array8 arr (V "arr") * [| length arr = 8|] ];;
+
+    "tmp" <- 0;;
+    [Al arr,
+      PREonly[V] mallocHeap 0 * [| V "arr" <> 0 |] * [| freeable (V "arr") 2 |]
+        * array8 arr (V "arr") * [| length arr = 8 |] ]
+    While ("tmp" < 8) {
+      Assert [Al arr,
+        PREonly[V] mallocHeap 0 * [| V "arr" <> 0 |] * [| freeable (V "arr") 2 |]
+        * array8 arr (V "arr") * [| length arr = 8 |] * [| (V "tmp" < natToW (length arr))%word |] ];;
+
+      "arr" + "tmp" *<-8 "tmp";;
+      "tmp" <- "tmp" + 1
+    };;
+
+    Call "array"!"inc"("arr", 8)
+    [Al arr, PREonly[V] mallocHeap 0 * [| V "arr" <> 0 |] * [| freeable (V "arr") 2 |]
+      * array8 arr (V "arr") * [| length arr = 8 |] ];;
+
+    "tmp" <-- Call "array"!"sum"("arr", 8)
+    [Al arr, PREonly[V] mallocHeap 0 * [| V "arr" <> 0 |] * [| freeable (V "arr") 2 |]
+      * array8 arr (V "arr") * [| length arr = 8 |] ];;
+
+    Call "sys"!"printInt"("tmp")
+    [Al arr, PREonly[V] mallocHeap 0 * [| V "arr" <> 0 |] * [| freeable (V "arr") 2 |]
+      * array8 arr (V "arr") * [| length arr = 8 |] ];;
+
+    Assert [Al arr, PREonly[V] mallocHeap 0 * [| V "arr" <> 0 |] * [| freeable (V "arr") 2 |]
+      * array8_decomission 2 arr (V "arr") * [| decomission_ok 2 arr |] ];;
+
+    Assert [PREonly[V] mallocHeap 0 * [| V "arr" <> 0 |] * [| freeable (V "arr") 2 |]
+      * V "arr" =?> 2];;
+
+    Call "malloc"!"free"(0, "arr", 2)
+    [PREonly[_] Emp];;
+
+    Call "sys"!"abort"()
+    [PREonly[_] [| False |] ]
   end
 }}.
 
@@ -303,6 +362,190 @@ Qed.
 
 Hint Rewrite sum_nil : sepFormula.
 
+Lemma materialize_array8'' : forall p v,
+  p =*> v ===> Ex b1, p =8> b1 * Ex b2, (p ^+ $1) =8> b2 * Ex b3, (p ^+ $2) =8> b3 * Ex b4, (p ^+ $3) =8> b4.
+  intros; hnf; unfold himp; intros.
+  unfold ptsto32, ptsto8, hptsto.
+  apply injL; intuition.
+  propxFo.
+  unfold smem_get_word, H.footprint_w in *.
+  
+  Require Import Bootstrap.
+
+  repeat match type of H0 with
+           | match ?E with None => _ | _ => _ end = _ => case_eq E; intros;
+             match goal with
+               | [ H : _ = _ |- _ ] => rewrite H in *
+             end; try discriminate
+         end.
+  do 4 esplit.
+  apply split_put_clear; [ apply split_a_semp_a | apply H ].
+  Local Hint Resolve get_put_eq get_put_ne get_emp.
+  intuition eauto.
+  rewrite get_put_ne; auto.
+  do 4 esplit.
+  apply split_put_clear; [ apply split_a_semp_a | ].
+  rewrite get_clear_ne; apply H2 || W_neq.
+  intuition eauto.
+  rewrite get_put_ne; auto.
+  do 4 esplit.
+  apply split_put_clear; [ apply split_a_semp_a | ].
+  rewrite get_clear_ne.
+  rewrite get_clear_ne; try apply H3.
+  W_neq.
+  W_neq.
+  intuition eauto.
+  rewrite get_put_ne; auto.
+  do 2 esplit.
+  rewrite get_clear_ne.
+  rewrite get_clear_ne.
+  rewrite get_clear_ne; try apply H4.
+  W_neq.
+  W_neq.
+  W_neq.
+  intros.
+  destruct (weq p' (p ^+ $2)); subst.
+  apply get_clear_eq.
+  rewrite get_clear_ne by auto.
+  destruct (weq p' (p ^+ $1)); subst.
+  apply get_clear_eq.
+  rewrite get_clear_ne by auto.
+  destruct (weq p' p); subst.
+  apply get_clear_eq.
+  rewrite get_clear_ne; eauto.
+Qed.
+
+Lemma materialize_array8' : forall p sz offset,
+  allocated p offset sz ===> Ex bs, array8 bs (p ^+ $(offset)) * [| (length bs = sz * 4)%nat |].
+  induction sz; simpl; intuition.
+  
+  sepLemma.
+  instantiate (1 := nil); auto.
+  sepLemma.
+
+  sepLemmaLhsOnly.
+  destruct offset.
+  etransitivity; [ eapply himp_star_frame; [ apply IHsz | apply materialize_array8'' ] | ].
+  sepLemmaLhsOnly.
+  fold (@length B) in *.
+  apply himp_ex_c; exists (x3 :: x2 :: x1 :: x0 :: x4).
+  sepLemma.
+  etransitivity; [ eapply himp_star_frame; [ apply IHsz | apply materialize_array8'' ] | ].
+  sepLemmaLhsOnly.
+  fold (@length B) in *.
+  apply himp_ex_c; exists (x3 :: x2 :: x1 :: x0 :: x4).
+  sepLemma.
+  match goal with
+    | [ |- himp _ (array8 _ ?X) (array8 _ ?Y) ] => replace Y with X; try reflexivity
+  end.
+  rewrite (natToW_S (S (S (S (S offset))))).
+  rewrite (natToW_S (S (S (S offset)))).
+  rewrite (natToW_S (S (S offset))).
+  rewrite (natToW_S (S offset)).
+  rewrite (natToW_S offset).
+  words.
+Qed.
+
+Theorem materialize_array8 : forall p sz,
+  p =?> sz ===> Ex bs, array8 bs p * [| (length bs = sz * 4)%nat |].
+  intros; eapply Himp_trans; [ apply materialize_array8' | ].
+  replace (p ^+ $0) with p by words.
+  apply Himp_refl.
+Qed.
+
+Lemma decomission_array8'' : forall p b1 b2 b3 b4,
+  (p =8> b1 * (p ^+ $1) =8> b2 * (p ^+ $2) =8> b3 * (p ^+ $3) =8> b4) ===> Ex w, p =*> w.
+  intros; hnf; unfold himp; intros.
+  unfold ptsto32, ptsto8, hptsto.
+  repeat ((apply existsL; intro) || (apply andL; (apply injL; intro) || (apply swap; apply injL; intro))).
+  apply injL; intuition.
+  propxFo.
+  do 2 esplit.
+  unfold smem_get_word, H.footprint_w.
+  repeat (erewrite split_smem_get; [ | | eauto ]).
+  eauto.
+  eauto.
+  eapply split_assoc.
+  apply split_comm; eauto.
+  eauto.
+  eapply split_assoc.
+  apply split_comm; eauto.
+  eapply split_assoc.
+  apply split_comm; eauto.
+  eauto.
+  eapply split_assoc.
+  apply split_comm; eauto.
+  eapply split_assoc.
+  apply split_comm; eauto.
+  apply split_comm; eauto.
+  intuition idtac.
+  unfold split in *; intuition subst.
+  repeat rewrite join_None; eauto.
+Qed.
+
+Lemma decomission_array8' : forall p sz bs offset sz',
+  length bs = sz' * 4
+  -> (sz' < sz)%nat
+  -> array8 bs (p ^+ $(offset)) ===> allocated p offset sz'.
+  induction sz; simpl; intuition.
+
+  destruct bs; simpl in *.
+  destruct sz'; simpl in *; try discriminate.
+  sepLemma.
+
+  destruct sz'; simpl in *; try discriminate.
+  do 3 (destruct bs; simpl in *; try discriminate).
+  replace (p ^+ $(offset) ^+ $1 ^+ $1 ^+ $1) with (p ^+ $(offset) ^+ $3) by words.
+  replace (p ^+ $(offset) ^+ $1 ^+ $1) with (p ^+ $(offset) ^+ $2) by words.
+
+  Lemma pull_out : forall P Q R S T,
+    P * (Q * (R * (S * T))) ===> (P * Q * R * S) * T.
+    sepLemma.
+  Qed.
+
+  eapply Himp_trans; [ apply pull_out | ].
+  apply Himp_star_frame.
+  eapply Himp_trans; [ apply decomission_array8'' | ].
+  destruct offset; sepLemma.
+  eapply Himp_trans; [ | apply IHsz ]; auto.
+  match goal with
+    | [ |- array8 _ ?X ===> array8 _ ?Y ] => replace Y with X; try apply Himp_refl
+  end.
+  change ($ (S (S (S (S offset))))) with (natToW (S (S (S (S offset))))).
+  rewrite (natToW_S (S (S (S offset)))).
+  rewrite (natToW_S (S (S offset))).
+  rewrite (natToW_S (S offset)).
+  rewrite (natToW_S offset).
+  unfold natToW.
+  W_eq.
+  congruence.
+Qed.
+
+Lemma decomission_array8 : forall p bs sz,
+  length bs = sz * 4
+  -> array8 bs p ===> p =?> sz.
+  intros; eapply Himp_trans; [ | eapply decomission_array8' ].
+  replace (p ^+ $0) with p by words; apply Himp_refl.
+  auto.
+  constructor.
+Qed.
+
+Theorem materialize_array8_tagged : forall p sz,
+  please_materialize sz
+  -> p =?> sz ===> Ex bs, array8 bs p * [| (length bs = sz * 4)%nat |].
+  intros; apply materialize_array8.
+Qed.
+
+Lemma decomission_array8_tagged : forall p bs sz,
+  decomission_ok sz bs
+  -> array8_decomission sz bs p ===> p =?> sz.
+  intros; apply decomission_array8; auto.
+Qed.
+
+Definition hints : TacPackage.
+  prepare (materialize_array8_tagged, decomission_array8_tagged) tt.
+Defined.
+
 Ltac useHyp := match goal with
                  | [ H : forall j : nat, _ |- _ ] => rewrite H by omega
                end.
@@ -324,7 +567,7 @@ Ltac finish :=
     | _ => eauto; reflexivity || words
   end.
 
-Ltac t :=
+Ltac t := solve [
   try match goal with
         | [ |- forall stn_st specs, interp _ _ -> interp _ _ ] =>
           match goal with
@@ -336,7 +579,22 @@ Ltac t :=
                       exists (done ++ mid :: nil); exists rem
               end
           end
-      end; sep_auto; finish.
+      end; sep hints; finish ].
+
+Opaque array8 allocated.
+
+Lemma length_inc : forall ls, length (inc ls) = length ls.
+  intros; apply map_length.
+Qed.
+
+Hint Rewrite length_inc : sepFormula.
+
+Lemma goodSize8 : forall n, n = 8
+  -> goodSize n.
+  intros; subst; auto.
+Qed.
+
+Hint Immediate goodSize8.
 
 Theorem ok : moduleOk m.
   vcgen; abstract t.
